SP1Clean/Proofs/Chips/LoadX0Chip/Witgen.lean
@@ -69,12 +69,11 @@ theorem computableWitnesses : (circuit (p := p)).base.ComputableWitnessesWithDat
     FlatOperation.forAll_witnessCongr_of_subcircuit _ _ ?_⟩
   · simp [circuit_norm]
   · have hob := Inputs.eval_congr_offset_bit h_input
-    simp only [eval_offsetBit] at hob
     simp only [circuit_norm]
     refine ⟨?_, ?_, ?_, ?_, ?_, ?_⟩
-    · have hv := Inputs.eval_congr_op_b_val h_input
+    · have hv := congrArg (fun r : Inputs (ZMod p) => r.op_b_val) h_input
       simpa only [eval_opBVal] using hv
-    · have hv := Inputs.eval_congr_op_c_imm h_input
+    · have hv := congrArg (fun r : Inputs (ZMod p) => r.op_c_imm) h_input
       simpa only [eval_opCImm] using hv
     · simpa [Vector.getElem_map] using congrArg (fun v : Vector (ZMod p) 3 => v[0]) hob
     · simpa [Vector.getElem_map] using congrArg (fun v : Vector (ZMod p) 3 => v[1]) hob
