SP1Clean/Proofs/Chips/StoreDoubleChip/Witgen.lean
@@ -49,9 +49,9 @@ theorem computableWitnesses : (circuit (p := p)).base.ComputableWitnessesWithDat
   · simp [circuit_norm]
   · simp only [circuit_norm]
     refine ⟨?_, ?_, ?_⟩
-    · have hv := Inputs.eval_congr_op_b_val h_input
+    · have hv := congrArg (fun r : Inputs (ZMod p) => r.op_b_val) h_input
       simpa only [eval_opBVal] using hv
-    · have hv := Inputs.eval_congr_op_c_imm h_input
+    · have hv := congrArg (fun r : Inputs (ZMod p) => r.op_c_imm) h_input
       simpa only [eval_opCImm] using hv
     · exact Inputs.eval_congr_is_real h_input
   all_goals simp [circuit_norm]
